compiler/dsl/coq/ReflexHVec.v
@@ -2,6 +2,46 @@ Require Import ReflexDenoted.
 Require Import ReflexFin.
 Require Import ReflexVec.
 
+Section SHeterogeneousVector.
+
+Variable desc : Set.
+Variable denote_desc : desc -> Set.
+
+Local Notation "[[ x ]]" := (denote_desc x).
+
+Fixpoint shvec (n : nat) : svec desc n -> Set :=
+  match n with
+  | O => fun _ => unit
+  | S n' => fun v =>
+    match v with
+    | (t, v') => [[ t ]] * shvec n' v'
+    end
+  end%type.
+
+Fixpoint shv_nth (n : nat) (v_d : svec desc n) (v : shvec n v_d) (i : fin n)
+  : [[ sv_get v_d i ]] :=
+  match n as _n return
+    forall (v_d : svec desc _n) (v : shvec _n v_d) (i : fin _n), [[ sv_get v_d i ]]
+  with
+  | O => fun v_d v i => match i with end
+  | S n' => fun (v_d : desc * svec desc n') (v : shvec (S n') v_d) i =>
+    match v_d as _v_d return
+      forall (v : shvec (S n') _v_d) (i : fin (S n')), [[ @sv_get desc (S n') _v_d i ]]
+    with
+    | (t, v_d') => fun (v : [[ t ]] * shvec n' v_d') (i : fin (S n')) =>
+      match i with
+      | None => fst v
+      | Some i' => shv_nth n' v_d' (snd v) i'
+      end
+    end v i
+  end v_d v i.
+
+End SHeterogeneousVector.
+
+Implicit Arguments shvec [desc n].
+
+Implicit Arguments shv_nth [desc n].
+
 Section HeterogeneousVector.
 
 Variable desc : Type.
