compiler/dsl/coq/ReflexVec.v
@@ -1,5 +1,33 @@
 Require Import ReflexFin.
 
+Section SVector.
+
+Variable T : Set.
+
+Check (unit * unit)%type.
+
+Fixpoint svec (n : nat) : Set :=
+  match n with
+  | O => unit
+  | S n' => T * svec n'
+  end%type.
+
+Fixpoint sv_get (n : nat) : svec n -> fin n -> T :=
+  match n with
+  | O => fun _ idx => match idx with end
+  | S n' => fun v idx =>
+    match idx with
+    | None => fst v
+    | Some idx' => sv_get n' (snd v) idx'
+    end
+  end.
+
+End SVector.
+
+Implicit Arguments sv_get [T n].
+
+(* keep that in case... *)
+
 Section Vector.
 
 Variable T : Type.
